Makefile
@@ -1,9 +1,21 @@
+COQLIB = /home/fbesson/.opam/coq-fajb/lib/coq/kernel
+
 all : CoqMakefile
 	make -f CoqMakefile
 
-prover :theories/Formula.v
-	find . -name prover.cmi -exec rm {} \;
-	find . -name prover.mli -exec rm {} \;
+src/prover.ml : theories/Formula.vo theories/Formula.v
+	cd theories ; coqc  Prover.v
+
+src/prover.cmx : src/prover.ml
+	rm -f src/prover.mli
+	ocamlopt -rectypes -c src/prover.ml -bin-annot -I $(COQLIB)
+
+
+src/proverPatch.ml : src/prover.cmx src/ppprover.ml
+	./src/patch/mlpatch -ifile src/prover.ml -pfile src/ppprover.ml > src/proverPatch.in
+	ocamlformat src/proverPatch.in > src/proverPatch.ml
+
+prover :  src/proverPatch.ml 
 
 install :
 	make -f CoqMakefile install
